rename to entails

LeanSAT/LRAT/Internal/Formula/Class.lean
@@ -3,7 +3,7 @@ Copyright Amazon.com, Inc. or its affiliates. All Rights Reserved.
 Released under Apache 2.0 license as described in the file LICENSE.
 Authors: Josh Clune
 -/
-import LeanSAT.LRAT.Internal.Sat
+import LeanSAT.LRAT.Internal.Entails
 import LeanSAT.LRAT.Clause
 
 namespace LRAT
@@ -12,7 +12,7 @@ open Std Sat
 
 /-- Typeclass for formulas. An instance [Formula α β σ] indicates that σ is
     the type of a formula with variables of type α, clauses of type β, and clause ids of type Nat -/
-class Formula (α : outParam (Type u)) (β : outParam (Type v)) [Clause α β] (σ : Type w) [HSat α σ] where
+class Formula (α : outParam (Type u)) (β : outParam (Type v)) [Clause α β] (σ : Type w) [Entails α σ] where
   toList : σ → List β -- A function used exclusively for defining Formula's satisfiability semantics
   readyForRupAdd : σ → Prop -- A predicate that indicates whether a formula can soundly be passed into performRupAdd
   readyForRatAdd : σ → Prop -- A predicate that indicates whether a formula can soundly be passed into performRatAdd
@@ -29,7 +29,7 @@ class Formula (α : outParam (Type u)) (β : outParam (Type v)) [Clause α β] (
     c ∈ toList (delete f arr) → c ∈ toList f
   delete_readyForRupAdd : ∀ f : σ, ∀ arr : Array Nat, readyForRupAdd f → readyForRupAdd (delete f arr)
   delete_readyForRatAdd : ∀ f : σ, ∀ arr : Array Nat, readyForRatAdd f → readyForRatAdd (delete f arr)
-  formulaHSat_def : ∀ p : α → Bool, ∀ f : σ, HSat.eval p f = (toList f).all (fun c => p ⊨ c)
+  formulaEntails_def : ∀ p : α → Bool, ∀ f : σ, Entails.eval p f = (toList f).all (fun c => p ⊨ c)
   performRupAdd : σ → β → Array Nat → σ × Bool
   rupAdd_result : ∀ f : σ, ∀ c : β, ∀ rupHints : Array Nat, ∀ f' : σ,
     readyForRupAdd f → performRupAdd f c rupHints = (f', true) → f' = insert f c
